examples/cms/gen_verif_full.sh
@@ -14,6 +14,10 @@ cp verif_Row11.v verif_Row14.v
 sed -i.bak 's/\["pipe"; "ingress"; "cm2_ds"; "win_1"; "row_1"\]/\["pipe"; "ingress"; "cm2_ds"; "win_1"; "row_4"\]/' verif_Row14.v
 rm verif_Row14.v.bak
 
+cp verif_Row11.v verif_Row15.v
+sed -i.bak 's/\["pipe"; "ingress"; "cm2_ds"; "win_1"; "row_1"\]/\["pipe"; "ingress"; "cm2_ds"; "win_1"; "row_5"\]/' verif_Row15.v
+rm verif_Row15.v.bak
+
 cp verif_Row11.v verif_Row21.v
 sed -i.bak 's/\["pipe"; "ingress"; "cm2_ds"; "win_1"; "row_1"\]/\["pipe"; "ingress"; "cm2_ds"; "win_2"; "row_1"\]/' verif_Row21.v
 rm verif_Row21.v.bak
@@ -29,6 +33,10 @@ rm verif_Row23.v.bak
 cp verif_Row11.v verif_Row24.v
 sed -i.bak 's/\["pipe"; "ingress"; "cm2_ds"; "win_1"; "row_1"\]/\["pipe"; "ingress"; "cm2_ds"; "win_2"; "row_4"\]/' verif_Row24.v
 rm verif_Row24.v.bak
+
+cp verif_Row11.v verif_Row25.v
+sed -i.bak 's/\["pipe"; "ingress"; "cm2_ds"; "win_1"; "row_1"\]/\["pipe"; "ingress"; "cm2_ds"; "win_2"; "row_5"\]/' verif_Row25.v
+rm verif_Row25.v.bak
 
 cp verif_Row11.v verif_Row31.v
 sed -i.bak 's/\["pipe"; "ingress"; "cm2_ds"; "win_1"; "row_1"\]/\["pipe"; "ingress"; "cm2_ds"; "win_3"; "row_1"\]/' verif_Row31.v
@@ -46,21 +54,9 @@ cp verif_Row11.v verif_Row34.v
 sed -i.bak 's/\["pipe"; "ingress"; "cm2_ds"; "win_1"; "row_1"\]/\["pipe"; "ingress"; "cm2_ds"; "win_3"; "row_4"\]/' verif_Row34.v
 rm verif_Row34.v.bak
 
-cp verif_Row11.v verif_Row41.v
-sed -i.bak 's/\["pipe"; "ingress"; "cm2_ds"; "win_1"; "row_1"\]/\["pipe"; "ingress"; "cm2_ds"; "win_4"; "row_1"\]/' verif_Row41.v
-rm verif_Row41.v.bak
-
-cp verif_Row11.v verif_Row42.v
-sed -i.bak 's/\["pipe"; "ingress"; "cm2_ds"; "win_1"; "row_1"\]/\["pipe"; "ingress"; "cm2_ds"; "win_4"; "row_2"\]/' verif_Row42.v
-rm verif_Row42.v.bak
-
-cp verif_Row11.v verif_Row43.v
-sed -i.bak 's/\["pipe"; "ingress"; "cm2_ds"; "win_1"; "row_1"\]/\["pipe"; "ingress"; "cm2_ds"; "win_4"; "row_3"\]/' verif_Row43.v
-rm verif_Row43.v.bak
-
-cp verif_Row11.v verif_Row44.v
-sed -i.bak 's/\["pipe"; "ingress"; "cm2_ds"; "win_1"; "row_1"\]/\["pipe"; "ingress"; "cm2_ds"; "win_4"; "row_4"\]/' verif_Row44.v
-rm verif_Row44.v.bak
+cp verif_Row11.v verif_Row35.v
+sed -i.bak 's/\["pipe"; "ingress"; "cm2_ds"; "win_1"; "row_1"\]/\["pipe"; "ingress"; "cm2_ds"; "win_3"; "row_5"\]/' verif_Row35.v
+rm verif_Row35.v.bak
 
 cp verif_Win1.v verif_Win2.v
 sed -i.bak 's/\["pipe"; "ingress"; "cm2_ds"; "win_1"\]/\["pipe"; "ingress"; "cm2_ds"; "win_2"\]/' verif_Win2.v
@@ -71,8 +67,3 @@ cp verif_Win1.v verif_Win3.v
 sed -i.bak 's/\["pipe"; "ingress"; "cm2_ds"; "win_1"\]/\["pipe"; "ingress"; "cm2_ds"; "win_3"\]/' verif_Win3.v
 sed -i.bak 's/verif_Row1/verif_Row3/' verif_Win3.v
 rm verif_Win3.v.bak
-
-cp verif_Win1.v verif_Win4.v
-sed -i.bak 's/\["pipe"; "ingress"; "cm2_ds"; "win_1"\]/\["pipe"; "ingress"; "cm2_ds"; "win_4"\]/' verif_Win4.v
-sed -i.bak 's/verif_Row1/verif_Row4/' verif_Win4.v
-rm verif_Win4.v.bak
